% declare document class and geometry
\documentclass[12pt]{article} % use larger type; default would be 10pt
\usepackage[margin=1in]{geometry} % handle page geometry

\input{../header2.tex}

\title{Phys 220A -- Classical Mechanics -- Lec06}
\author{UCLA, Fall 2014}
\date{\formatdate{21}{10}{2014}} % Activate to display a given date or no date (if empty),
         % otherwise the current date is printed 

\begin{document}
\setlength{\unitlength}{1mm}
\maketitle


\section{Small oscillations}

Generally, in classical mechanics, the dynamics may often by too complicated to solve exactly, or even numerically. Often we will have a Lagrangian of the form
\begin{eqn}
L = \frac{1}{2} \sum_{ij} M_{ij}(q) \dot{q}_i \dot{q}_j + \sum_i N_i (q) \dot{q}_i - V(q),
\end{eqn}
or we will be able to approximate it in this form to order $\bigo(\dot{q}^2)$, assuming no time dependence. This gives us stability around equilibrium, which is of course important physically. An example where $N_i$ comes into play would be the potential for a particle coupled to the EM field. For driven systems we will have different stability properties. In condensed matter, small energy excitations around equilibrium are called phonons. 

Equilibrium points occur at the extrema of the potential, that is at solutions $q_i^{(0)}$ to $\pd{V}{q_i} = 0$. The Euler-Lagrange equations are then solved by $q_i(t) = q_i^{(0)}$ for all $t$, i.e. $\dot{q}_i = 0$. Under small oscillations we will have
\begin{eqn}
q_i = q_i^{(0)} + \eta_i(t) + \bigo(\eta^2)
\end{eqn}
and we must expand the Lagrangian to quadratic order (i.e. linearize),
\begin{align}
L &= \frac{1}{2} \sum_{ij} M_{ij} (q^{0}) \dot{\eta}_i \dot{\eta}_j + \sum_i N_i (q^{0}) \dot{\eta}_i + \sum_{ij} \eval{\pd{N_i}{q_j}}_{q=q^0} \eta_j \dot{\eta}_i - V(q^0) \\
	& \qquad - \sum_i \eval{\pd{V}{q_i}}_{q = q^0} \eta_i - \frac{1}{2} \eval{\md{V}{2}{q_i}{}{q_j}{}}_{q = q^0} \eta_i \eta_j + \bigo(n^3). \\
	&\sim \frac{1}{2} \sum_{ij} m_{ij} \dot \eta_i \dot \eta_j - \frac{1}{2} \sum_{ij} v_{ij} \eta_i \eta_j + \sum_{ij} p_{ij} \eta_i \dot \eta_j + \bigo(\eta^3),
\end{align}
where in the second expression we've thrown out the $\sum_i N_i (q^0) \dot{\eta}_i$ and $V(q^0)$ terms since they are just a total derivative and an overall constant, and 
\begin{eqn}
m_{ij} = M_{ij}(q^0), \qquad p_{ij} = \eval{\pd{N_i}{q_j}}_{q = q^0}, \text{and} \qquad v_{ij} = \eval{\md{V}{2}{q_i}{}{q_j}{}}_{q = q^0}
\end{eqn}
are constant matrices. Now, if $p_{ij}$ has a symmetric part $p_{(ij)}$ we can throw it out and just consider it antisymmetric since
\begin{eqn}
p_{(ij)} \eta_i \dot{\eta}_j = \frac{1}{2} (p_{ij} + p_{ji}) \eta_i \dot{\eta}_j = p_{ij} (\eta_i \dot{\eta}_j + \eta_j \dot{\eta}_i) = \od{}{t} (\frac{1}{2} p_{ij} \eta_i \eta_j)
\end{eqn}
is just a total derivative. 

\subsection{First analysis}

As a first analysis, let's set $p_{ij} = 0$. Then we can write
\begin{eqn}
L = \frac{1}{2} \dot{\eta}^\top m \dot{\eta} - \frac{1}{2} \eta^\top v \eta + \bigo(\eta^3),
\end{eqn}
for which we can write the equation of motion in terms of the vector $\bar{\eta} = (\eta_1, \dots, \eta_n)$,
\begin{eqn}
m \ddot{\bar{\eta}} + v \bar{\eta} = 0.
\end{eqn}
This has ansatz $\bar{\eta} = \bar{\gamma} e^{i \omega t}$ which, plugging back in to the equation of motion, we have
\begin{eqn}
(-\omega^2 m + v) \bar{\gamma} = 0.
\end{eqn}
Thus $\omega$ is determined by the vanishing of the determinant
\begin{eqn}
\det (-\omega^2 m + v) = 0.
\end{eqn}

[blah blah, incomplete here]


Thus our equatons of motion are given by
\begin{eqn}
\ddot{\bbar{\eta}}_i + \lambda_i \bbar{\eta}_i = 0, \qquad i = 1, \dots, N.
\end{eqn}
where in the stable case we have $\lambda_i = \omega_i^2$, the characteristic frequencies. So the normal modes are decoupled 1-dimensional oscillators along $\bbar{\eta}_i$ with coordinate relationship
\begin{eqn}
\eta = O \bar{m}^{-1/2} \bar{O} \bar{\bar{\eta}}. 
\end{eqn}

In the more general case with $\eta_{ij} \neq 0$, we have
\begin{eqn}
L = \frac{1}{2} \dot{\bar{\eta}}^\top \bar{\eta} + \bar{\eta}^\top \bar{p} \dot{\bar{\eta}} - \frac{1}{2} \bar{\eta}^\top \bar{v} \bar{\eta}
\end{eqn}
where
\begin{eqn}
\bar{p} = \bar{m}^{-1/2} O^\top p O \bar{m}^{-1/2}.
\end{eqn}
So the Euler-Lagrange equations are
\begin{eqn}
\ddot{\bar{\eta}} + \bar{v} \bar{\eta} - 2 \bar{p} \dot{\bar{\eta}} = 0
\end{eqn}
which has a new characteristic equation for the ansatz $\bar{\eta} = \gamma e^{i\omega t}$,
\begin{eqn}
\det (-\omega^2 + \bar{v} - 2i \omega \bar{p}) = 0
\end{eqn}
which determines $\omega$ and $\gamma$ in general. These cases are important for a particle in an EM field and motion in non-inertial frames. 


\subsection{Double pendulum}

[unfinished]





\end{document}
