% declare document class and geometry
\documentclass[12pt]{article} % use larger type; default would be 10pt
\usepackage[margin=1in]{geometry} % handle page geometry

\input{../header2.tex}

\title{Phys 220A -- Classical Mechanics -- Lec10}
\author{UCLA, Fall 2014}
\date{\formatdate{6}{11}{2014}} % Activate to display a given date or no date (if empty),
         % otherwise the current date is printed 

\begin{document}
\setlength{\unitlength}{1mm}
\maketitle


\section{Symplectic Geometry}

If we want to write the Poisson bracket for some arbitrary functions, i.e.
\begin{eqn}
C(q,p) = \cbr{A(q,p), B(q,p)},
\end{eqn}
we can expand in $q, p$ and we find that the fundamental bracket is really the ``canonical'' coordinate brackets,
\begin{eqn}
\cbr{q_i, q_j} = 0, \qquad
\cbr{p_i, p_j} = 0, \qquad
\cbr{q_i, p_j} = \delta_{ij}.
\end{eqn}
We see that (as expected from quantum-classical correspondence) these are basically the same as in quantum mechanics just without the factor of $i\hbar$. 

If we write points in phase space using aggregate coordinates 
\begin{eqn}
\xi_I = (q_1, \dots, q_n, p_1, \dots, p_n)^\top,
\end{eqn}
we can reformulate Hamilton's equations as a single differential equation
\begin{eqn}
\dot \xi_I = \sum_J J_{IJ} \pd{H}{\xi_J}, \qquad
J = \pmat{0 & 1_n \\ -1_n & 0}.
\end{eqn}
Suppose we have a coordinate transformation
\begin{eqn}
Q = Q(q,p), \qquad P = P(q,p).
\end{eqn}
If this transformation leaves the structure of Hamilton's equations unchanged, i.e. it leaves the symplectic geometry invariant, we call it a canonical transformation. We can characterize canonical transformations in a few equivalent ways as follows.
\begin{enumerate}
\item Structure of Hamilton's equations is unchanged:
\begin{eqn}
H'(P,Q) = H(q(Q,P), p(Q,P))
\end{eqn}
we will have
\begin{eqn}
\dot P = -\pd{H'}{Q}, \qquad
\dot Q = \pd{H'}{P}.
\end{eqn}
\item Poisson brackets are invariant:
\begin{eqn}
\cbr{A'(Q,P), B'(Q,P)}_{QP} = \cbr{A(q,p), B(q,p)}_{qp}.
\end{eqn}
\item Under the transformation $Y_I = Y_I(X_I)$, the matrix $J_{IJ}$ can be written in terms of the Jacobian $j_{IJ}$ as
\begin{eqn}
J = j J j^\top, \qquad
J_{IJ} = \sum_{KL} \pd{Y_I}{X_K} J_{KL} \pd{Y_J}{X_L}.
\end{eqn}
\item Most importantly: the Poisson brackets of the new coordinates are canonical,
\begin{eqn}
\cbr{Q_i, Q_j}_{qp} = 0, \qquad
\cbr{P_i, P_j}_{qp} = 0, \qquad
\cbr{Q_i, P_j}_{qp} = \delta_{ij}.
\end{eqn}
\end{enumerate}

We can show that that canonical transformations reproduce Hamilton's equations [which characterization?]. We know
\begin{eqn}
\dot X_I = \sum_J J_{IJ} \pd{H}{X_J} = \sum_J \pd{X_I}{Y_J} \dot Y_J,
\end{eqn}
and also
\begin{eqn}
\pd{H}{X_J} = \sum_K \pd{H'}{Y_K} \pd{Y_K}{X_J}.
\end{eqn}
Then we find that
\begin{eqn}
\sum_J \dot Y_J \pd{X_I}{Y_J} = \sum_{J,K} J_{IJ} \pd{H'}{Y_K} \pd{Y_K}{X_J}
\end{eqn}
and using
\begin{eqn}
\sum_I \pd{X_I}{Y_J} \pd{Y_K}{X_I} = \delta_{KJ}
\end{eqn}
we multiply both sides by $\pd{Y_M}{X_I}$ and sum over $I$ to find
\begin{eqn}
\sum_J \dot Y_J \delta_{MJ} 
	= \sum_{IJK} \pd{Y_M}{X_I} J_{IJ} \pd{Y_K}{X_J} \pd{H'}{Y_K} 
	= \sum_K J_{MK} \pd{H'}{Y_K}.
\end{eqn}


\subsection{Some Examples of Canonical Transformations}

\begin{example}
Suppose we have the transformation $Q = p$, $P = -q$. Then
\begin{eqn}
\cbr{Q,P}_{qp} = - \cbr{p,q} = +1.
\end{eqn}
So this is a very simple example of a canonical transformation that shows how the $q$s and $p$s are really somewhat interchangeable. For example if we have a relativistic harmonic oscillator
\begin{eqn}
H = \sqrt{p^2 + m^2} + \frac{1}{2} m \omega^2 q^2,
\end{eqn}
under the transformation this is just
\begin{eqn}
H' = \sqrt{Q^2 + m^2} + \frac{1}{2} m \omega^2 P^2.
\end{eqn}
\end{example}

\begin{example}
Consider the transformation [this was on the final last year]
\begin{eqn}
Q = \frac{1}{2} p^2, \qquad
P = -\frac{p}{q},
\end{eqn}
so that
\begin{eqn}
p = \sqrt{2Q}, \qquad
q = -\sqrt{2Q} P.
\end{eqn}
Then we have
\begin{eqn}
\cbr{Q,P} = \frac{1}{2} \left( \pd{(p^2)}{q} \pd{(-q/p)}{p} - \pd{(p^2)}{p} \pd{(-q/p)}{q} \right) = p \frac{1}{p} = 1.
\end{eqn}
Then 
\begin{eqn}
H = p^2 + q^2, \qquad
H' = 2Q + 2QP^2.
\end{eqn}
\end{example}

This approach can be somewhat messy but there it turns out that there is a nicer, more algorithmic way of checking for canonical transformations. This is the method of generating functions. 


\subsection{Method of generating functions}

In this method, we will pick out functions of one old coordinate and one new coordinate so that, for example for some function $F_1(q,Q,t)$
\begin{eqn}
p = \eval{\pd{F_1}{q}}_Q \qquad \implies \qquad Q = Q(q,p),
\end{eqn}
and
\begin{eqn}
P = -\eval{\pd{F_1}{Q}}_q \qquad \implies \qquad P = P(q,p),
\end{eqn}
since
\begin{eqn}
\eval{\pd{P}{p}}_q = \eval{\pd{P}{Q}}_q \eval{\pd{Q}{p}}_q.
\end{eqn}
We will need to do this for four functions $F_1, F_2, F_3, F_4$ with parameters as all four combinations of $q,p$ and $Q,P$.

\begin{proof}
Recall that we can write the action
\begin{eqn}
S = \int \dif{t} (p \dot q - H),
\end{eqn}
so for some transformed coordinates we can write
\begin{eqn}
S = \int \dif t (P \dot Q - K)
\end{eqn}
for some function $K(Q,P)$ which will just be $H'(Q,P)$ for a canonical transformation. This is sometimes referred to as the "Cameltoenian". So we want
\begin{align}
p \dot q - H &= P \dot Q - K(Q,P) + \dod{}{t} F_1(q,Q) \\
	&= P \dot Q - K(Q, P) + \dpd{F_1}{t} + \dpd{F_1}{q} \dot q + \dpd{F_1}{Q} \dot Q.
\end{align}
So we have what we want if
\begin{eqn}
p = \pd{F_1}{q}, \qquad
P = -\pd{F_1}{Q}, \qquad
K = H + \pd{F_1}{t}.
\end{eqn}
\end{proof}

So for the three other functions we will have
\begin{eqn}
F_2(q,P), \qquad p = \pd{F_2}{q}, \qquad Q = \pd{F_2}{p},
\end{eqn} \begin{eqn}
F_3(p,Q), \qquad q = -\pd{F_3}{p}, \qquad P = -\pd{F_3}{Q},
\end{eqn} \begin{eqn}
F_4(p,P), \qquad q = -\pd{F_4}{p}, \qquad Q = \pd{F_4}{P}.
\end{eqn}

\setcounter{example}{0}
\begin{example}
Let $F_1 = qQ$, then
\begin{eqn}
p = \pd{F_1}{q} = Q, \qquad P = -\pd{F_1}{Q} = -q, \qquad H = K.
\end{eqn}
\end{example}

\begin{example}
Given Hamiltonian
\begin{eqn}
H = \frac{p^2}{2m} + \frac{1}{2} m \omega^2 q^2,
\end{eqn}
using 
\begin{eqn}
F_1 = \frac{m \omega}{2} q^2 \cot Q,
\end{eqn}
we find
\begin{eqn} 
p = m \omega q \cot Q, \qquad
P = \frac{m \omega q^2}{2 \sin^2 Q}.
\end{eqn}
so that
\begin{eqn}
q = \sqrt{\frac{2P}{m\omega}} \sin Q, \qquad
p = \sqrt{2 m \omega P} \cos Q,
\end{eqn}
and
\begin{eqn}
K = \omega P (\sin^2 Q + \cos^2 Q) = \omega P.
\end{eqn}
This one in particular is useful if $Q$ is cyclic and $P$ is constant, in which case $Q = Q_0 + \omega t$.
\end{example}








\end{document}
